Let $\hat{\Omega}$ be the pole of rotation. Convenience justifies aligning it with the $\hat{z}$ axis.
Let $\hat{M}$ be the magnetic axis, pointing in an arbitrary direction.
Let $\hat{k}$ be the line of sight vector, which we place for the sake of convenience, in the $xz$ plane.

Then we have the following Cartesian definitions:
$$
\begin{align}
	\hat{\Omega} &= \hat{z}\\
	\hat{M} &= \sin{\alpha} \cos{\varphi} \, \hat{x} + \sin{\alpha} \sin{\varphi} \, \hat{y} + \cos{\alpha} \, \hat{z}\\
	\hat{k} &= \sin{\xi} \, \hat{x} + \cos{\xi} \, \hat{z}
\end{align}
$$

Step 1: Define the plane tangent to the surface at the line of sight vector $\hat{k}$.

In this plane, the unit $n$ and $m$ vectors can be defined as follows:
$$
\begin{align}
	\hat{n_1} &= \frac{\hat{\Omega}-(\hat{\Omega} \cdot \hat{k}) \hat{k}}{|\hat{\Omega}-(\hat{\Omega} \cdot \hat{k}) \hat{k}|}\\
	\hat{n_2} &= \frac{\hat{M}-(\hat{M} \cdot \hat{k}) \hat{k}}{|\hat{M}-(\hat{M} \cdot \hat{k}) \hat{k}|}\\
	\hat{m_1} &= \hat{n_1} \times \hat{k}\\
	\hat{m_2} &= \hat{n_2} \times \hat{k}
\end{align}
$$

Step 2: In this plane, we find the vectors $\hat{n_1}$ and $\hat{n_2}$, which point to the axis of rotation and the magnetic pole, respectively. Then we also find the perpendicular auxiliary vectors $\hat{m_1}$ and $\hat{m_2}$.

#### Finding $\hat{n_1}$
$$
\begin{align}
	\hat{\Omega} \cdot \hat{k} &= \cos{\xi}\\
	\hat{\Omega} - (\hat{\Omega} \cdot \hat{k})\hat{k} &= \hat{z} - \sin{\xi} \cos{\xi}\,\hat{x} - \cos^2{\xi}\,\hat{z}\\ &= -\sin{\xi} \cos{\xi}\,\hat{x} + \sin^2{\xi}\,\hat{z}\\
	|\hat{\Omega} - (\hat{\Omega} \cdot \hat{k})\hat{k}| &= \sqrt{\sin^2{\xi} \cos^2{\xi} + \sin^4{\xi}} = \sin{\xi}\\
	\hat{n_1} &= \frac{\hat{\Omega}-(\hat{\Omega} \cdot \hat{k}) \hat{k}}{|\hat{\Omega}-(\hat{\Omega} \cdot \hat{k}) \hat{k}|}\\ &= -\frac{\sin{\xi} \cos{\xi}\,\hat{x} + \sin^2{\xi}\,\hat{z}}{\sin{\xi}}\\\\ 
	\hat{n_1} &= -\cos{\xi}\,\hat{x} + \sin{\xi}\,\hat{z}
\end{align}
$$

#### Finding $\hat{m_1}$
$$
\begin{align}
	\hat{n_1} &= -\cos{\xi}\,\hat{x} + \sin{\xi}\,\hat{z}\\
	\hat{k} &= \sin{\xi}\,\hat{x} + \cos{\xi}\,\hat{z}
\end{align}
$$$$
\begin{align}
	\hat{m_1} &= \hat{n_1} \times \hat{k} = (n_y k_z - n_z k_y)\hat{x} - (n_x k_z - n_z k_x)\hat{y} + (n_x k_y - n_y k_x)\hat{z}\\ &= (n_z k_x - n_x k_z)\hat{y} = (\sin^2{\xi}+\cos^2{\xi})\,\hat{y} = \hat{y}\\\\
	\hat{m_1} &= \hat{y}
\end{align}
$$

#### Finding $\hat{n_2}$
$$
\begin{align}
	\hat{M} &= \sin{\alpha} \cos{\varphi} \, \hat{x} + \sin{\alpha} \sin{\varphi} \, \hat{y} + \cos{\alpha} \, \hat{z}\\
	\hat{k} &= \sin{\xi} \, \hat{x} + \cos{\xi} \, \hat{z}
\end{align}
$$

$$
\begin{align}
	\hat{M} \cdot \hat{k} &= \sin{\xi} \sin{\alpha} \cos{\varphi} + \cos{\xi} \cos{\alpha} = \cos{\Gamma}\\
	\hat{M}-(\hat{M}\cdot\hat{k})\hat{k} &= \sin{\alpha}\cos{\varphi}\,\hat{x} + \sin{\alpha} \sin{\varphi}\,\hat{y} + \cos{\alpha}\,\hat{z} - \cos{\Gamma}\sin{\xi}\,\hat{x} - \cos{\Gamma}\cos{\xi}\,\hat{z}\\
	&= (\sin{\alpha}\cos{\varphi}-\cos{\Gamma}\sin{\xi})\hat{x}+(\sin{\alpha}\sin{\varphi})\hat{y}+(\cos{\alpha}-\cos{\Gamma}\cos{\xi})\hat{z}\\
	|\hat{M}-(\hat{M}\cdot\hat{k})\hat{k}|^2 &= (\sin{\alpha}\cos{\varphi}-\cos{\Gamma}\sin{\xi})^2+(\sin{\alpha}\sin{\varphi})^2+(\cos{\alpha}-\cos{\Gamma}\cos{\xi})^2\\
	&= \sin^2{\alpha}\cos^2{\varphi} + \cos^2{\Gamma}\sin^2{\xi}-2\sin{\alpha}\cos{\varphi}\sin{\xi}\cos{\Gamma}\\
	&+ \sin^2{\alpha}\sin^2{\varphi} + \cos^2{\alpha} + \cos^2{\xi}\cos^2{\Gamma}-2\cos{\alpha}\cos{\xi}\cos{\Gamma}\\
	&= 1 + \cos^2{\Gamma} - 2\cos{\Gamma}(\sin{\xi}\sin{\alpha}\cos{\varphi}+\cos{\xi}\cos{\alpha})\\
	&= 1 + \cos^2{\Gamma} - 2\cos^2{\Gamma} = 1 - \cos^2{\Gamma} = \sin^2{\Gamma}\\
	|\hat{M}-(\hat{M}\cdot\hat{k})\hat{k}| &= \sin{\Gamma}\\\\
	\hat{n_2} &= \frac{(\sin{\alpha}\cos{\varphi}-\cos{\Gamma}\sin{\xi})\hat{x} + (\sin{\alpha}\sin{\varphi})\hat{y} + (\cos{\alpha}-\cos{\Gamma}\cos{\xi})\hat{z}}{\sin{\Gamma}}
\end{align}
$$

#### Finding $\hat{m_2}$
$$
\begin{align}
	\hat{n_2} &= \frac{(\sin{\alpha}\cos{\varphi}-\cos{\Gamma}\sin{\xi})\hat{x} + (\sin{\alpha}\sin{\varphi})\hat{y} + (\cos{\alpha}-\cos{\Gamma}\cos{\xi})\hat{z}}{\sin{\Gamma}}\\
	\hat{k} &= \sin{\xi}\,\hat{x} + \cos{\xi}\,\hat{z}
\end{align}
$$

$$
\begin{align}
\hat{m_2} &= \hat{n_1} \times \hat{k} = (n_y k_z - n_z k_y)\hat{x} - (n_x k_z - n_z k_x)\hat{y} + (n_x k_y - n_y k_x)\hat{z}\\\\
&= \frac{\cos{\xi}\sin{\alpha}\sin{\varphi}}{\sin{\Gamma}}\,\hat{x}\\ &+  \frac{\sin{\xi}(\cos{\alpha}-\cos{\Gamma}\cos{\xi})-\cos{\xi}(\sin{\alpha}\cos{\varphi}-\cos{\Gamma}\sin{\xi})}{\sin{\Gamma}}\,\hat{y}\\ &- \frac{\sin{\xi}\sin{\alpha}\sin{\varphi}}{\sin{\Gamma}}\,\hat{z}
\end{align}
$$

Step 3: Find $\cos{\chi}$ and $\sin{\chi}$.

#### Finding $\cos{\chi}$
$$
\begin{align}
\hat{n_1} &= -\cos{\xi}\,\hat{x} + \sin{\xi}\,\hat{z}\\
\hat{n_2} &= \frac{(\sin{\alpha}\cos{\varphi}-\cos{\Gamma}\sin{\xi})\hat{x} + (\sin{\alpha}\sin{\varphi})\hat{y} + (\cos{\alpha}-\cos{\Gamma}\cos{\xi})\hat{z}}{\sin{\Gamma}}
\end{align}
$$
$$
\begin{align}
\cos{\chi} &= \hat{n_1}\cdot\hat{n_2}\\
&= \frac{-\cos{\xi}(\sin{\alpha}\cos{\varphi}-\cos{\Gamma}\sin{\xi}) + \sin{\xi}(\cos{\alpha}-\cos{\Gamma}\cos{\xi})}{\sin{\Gamma}}\\
&= \frac{\sin{\xi}\cos{\xi}\cos{\Gamma}-\cos{\xi}\sin{\alpha}\cos{\varphi}-\sin{\xi}\cos{\xi}\cos{\Gamma}+\sin{\xi}\cos{\alpha}}{\sin{\Gamma}}\\\\
\cos{\chi} &= \frac{\sin{\xi}\cos{\alpha}-\cos{\xi}\sin{\alpha}\cos{\varphi}}{\sin{\Gamma}}
\end{align}
$$


#### Finding $\sin{\chi}$
$$
\begin{align}
\hat{n_1} &= -\cos{\xi}\,\hat{x}+\sin{\xi}\,\hat{z}\\\\
\hat{m_2} &= \frac{\cos{\xi}\sin{\alpha}\sin{\varphi}}{\sin{\Gamma}}\,\hat{x}\\ &+  \frac{\sin{\xi}(\cos{\alpha}-\cos{\Gamma}\cos{\xi})-\cos{\xi}(\sin{\alpha}\cos{\varphi}-\cos{\Gamma}\sin{\xi})}{\sin{\Gamma}}\,\hat{y}\\ &- \frac{\sin{\xi}\sin{\alpha}\sin{\varphi}}{\sin{\Gamma}}\,\hat{z}\\\\
\hat{n_2} &= \frac{(\sin{\alpha}\cos{\varphi}-\cos{\Gamma}\sin{\xi})\hat{x} + (\sin{\alpha}\sin{\varphi})\hat{y} + (\cos{\alpha}-\cos{\Gamma}\cos{\xi})\hat{z}}{\sin{\Gamma}}\\\\
\hat{m_1} &= \hat{y}
\end{align}
$$
$$
\begin{align}
\sin{\chi} &= \hat{m_2}\cdot\hat{n_1}=-\hat{m_1}\cdot\hat{n_2}\\\\
-\hat{m_1}\cdot\hat{n_2} &= -\frac{\sin{\alpha}\sin{\varphi}}{\sin{\Gamma}}\\\\
\hat{m_2}\cdot\hat{n_1} &= -\frac{\cos^2{\xi}\sin{\alpha}\sin{\varphi}}{\sin{\Gamma}}-\frac{\sin^2{\xi}\sin{\alpha}\sin{\varphi}}{\sin{\Gamma}}\\\\
&= -\frac{1}{\sin{\Gamma}}[\sin{\alpha}\sin{\varphi}(\cos^2{\xi}+\sin^2{\xi})]\\\\
&= -\frac{\sin{\alpha}\sin{\varphi}}{\sin{\Gamma}}
\end{align}
$$

Step 4: Find $\tan{\chi}$.

#### Finding $\tan{\chi}$
$$
\begin{align}
\sin{\chi} &= -\frac{\sin{\alpha}\sin{\varphi}}{\sin{\Gamma}}\\\\
\cos{\chi} &= \frac{\sin{\xi}\cos{\alpha}-\cos{\xi}\sin{\alpha}\cos{\varphi}}{\sin{\Gamma}}\\\\
\tan{\chi} &= \frac{\sin{\chi}}{\cos{\chi}} = -\frac{\sin{\alpha}\sin{\varphi}}{\sin{\Gamma}} \cdot \frac{\sin{\Gamma}}{\sin{\xi}\cos{\alpha}-\cos{\xi}\sin{\alpha}\cos{\varphi}}\\\\
&= \frac{\sin{\alpha}\sin{\varphi}}{\cos{\xi}\sin{\alpha}\cos{\varphi}-\sin{\xi}\cos{\alpha}}
\end{align}
$$